hax-lib/proof-libs/lean/Hax/MissingLean/Init/Data/UInt/Lemmas.lean
@@ -14,6 +14,19 @@ attribute [grind =_] UInt16.le_ofNat_iff
 attribute [grind =_] UInt32.le_ofNat_iff
 attribute [grind =_] UInt64.le_ofNat_iff
 
+@[grind =]
+theorem UInt64.toNat_add_of_lt {a b : UInt64} (h : a.toNat + b.toNat < 2 ^ 64) :
+    (a + b).toNat = a.toNat + b.toNat := by
+  rw [UInt64.toNat_add, Nat.mod_eq_of_lt h]
+
+theorem UInt64.succ_le_of_lt {a b : UInt64} (h : a < b) :
+    a + 1 ≤ b := by grind
+
+theorem UInt64.add_le_of_le {a b c : UInt64} (habc : a + b ≤ c) (hab : a.toNat + b.toNat < 2 ^ 64):
+    a ≤ c := by
+  rw [UInt64.le_iff_toNat_le, UInt64.toNat_add_of_lt hab] at *
+  omega
+
 @[grind]
 theorem USize.umulOverflow_iff (x y : USize) :
     BitVec.umulOverflow x.toBitVec y.toBitVec ↔ x.toNat * y.toNat ≥ 2 ^ System.Platform.numBits :=
@@ -25,16 +38,16 @@ theorem USize.uaddOverflow_iff (x y : USize) :
   by simp [BitVec.uaddOverflow]
 
 @[grind =]
-theorem USize.toNat_mul_of_lt (a b : USize) (h : a.toNat * b.toNat < 2 ^ System.Platform.numBits) :
+theorem USize.toNat_mul_of_lt {a b : USize} (h : a.toNat * b.toNat < 2 ^ System.Platform.numBits) :
     (a * b).toNat = a.toNat * b.toNat := by
   rw [USize.toNat_mul, Nat.mod_eq_of_lt h]
 
 @[grind =]
-theorem USize.toNat_add_of_lt (a b : USize) (h : a.toNat + b.toNat < 2 ^ System.Platform.numBits) :
+theorem USize.toNat_add_of_lt {a b : USize} (h : a.toNat + b.toNat < 2 ^ System.Platform.numBits) :
     (a + b).toNat = a.toNat + b.toNat := by
   rw [USize.toNat_add, Nat.mod_eq_of_lt h]
 
 @[grind ←]
-theorem USize.le_self_add (a b : USize) (h : a.toNat + b.toNat < 2 ^ System.Platform.numBits) :
+theorem USize.le_self_add {a b : USize} (h : a.toNat + b.toNat < 2 ^ System.Platform.numBits) :
     a ≤ a + b := by
   grind
